Wavelet/Semantics.lean
@@ -2,5 +2,6 @@ import Wavelet.Semantics.Defs
 import Wavelet.Semantics.Lts
 import Wavelet.Semantics.Link
 import Wavelet.Semantics.OpInterp
+import Wavelet.Semantics.PCM
 
 /-! Common definitions for semantics. -/
