Wavelet/Semantics/PCM.lean
@@ -1,0 +1,41 @@
+/-! Definitions for PCM. -/
+
+namespace Wavelet.Semantics
+
+class PCM (C : Type u) where
+  add : C → C → C
+  zero : C
+  valid : C → Prop
+  eq : C → C → Prop
+
+infixl:60 " ⊔ " => PCM.add
+infix:40 " ≡ " => PCM.eq
+prefix:40 "✓ " => PCM.valid
+
+def PCM.disjoint {C : Type u} [PCM C] (a b : C) : Prop := ✓ a ⊔ b
+
+/-- TODO: Implement some type class for partial order. -/
+def PCM.le {C : Type u} [PCM C] (a b : C) : Prop := ∃ c, b ≡ a ⊔ c
+
+noncomputable def PCM.sub {C : Type u} [PCM C] (a b : C) (hle : PCM.le a b) : C :=
+  hle.choose
+
+def PCM.framePreserving {C : Type u} [PCM C] (a b : C) : Prop :=
+  ∀ c, ✓ a ⊔ c → ✓ b ⊔ c
+
+infix:50 " ⊥ " => PCM.disjoint
+infix:50 " ≤ " => PCM.le
+infix:50 " ⟹ " => PCM.framePreserving
+
+class LawfulPCM (R : Type u) [inst : PCM R] where
+  add_comm : ∀ a b : R, a ⊔ b ≡ b ⊔ a
+  add_assoc : ∀ a b c : R, (a ⊔ b) ⊔ c ≡ a ⊔ (b ⊔ c)
+  add_ident : ∀ a : R, a ⊔ inst.zero ≡ a
+  valid_add : ∀ a b : R, ✓ a ⊔ b → ✓ a
+  valid_zero : ✓ inst.zero
+  valid_eq : ∀ a b : R, a ≡ b → ✓ a → ✓ b
+  eq_refl : ∀ a : R, a ≡ a
+  eq_symm : ∀ a b : R, a ≡ b → b ≡ a
+  eq_trans : ∀ a b c : R, a ≡ b → b ≡ c → a ≡ c
+
+end Wavelet.Semantics
